cedar-lean/Cedar/Thm/Partial/Evaluation.lean
@@ -15,8 +15,10 @@
 -/
 
 import Cedar.Partial.Evaluator
+import Cedar.Partial.Expr
 import Cedar.Spec.Evaluator
 import Cedar.Thm.Partial.Evaluation.And
+import Cedar.Thm.Partial.Evaluation.AndOr
 import Cedar.Thm.Partial.Evaluation.Basic
 import Cedar.Thm.Partial.Evaluation.Binary
 import Cedar.Thm.Partial.Evaluation.Call
@@ -141,3 +143,214 @@ theorem on_concrete_gives_concrete (expr : Spec.Expr) (request : Spec.Request) (
   <;> split at h
   <;> simp only [Except.ok.injEq, Except.error.injEq, Partial.Value.value.injEq] at h
   <;> trivial
+
+/--
+  If partial evaluation returns a concrete value, then it returns the same value
+  after any substitution of unknowns
+-/
+theorem subst_preserves_evaluation_to_value {expr : Partial.Expr} {req req' : Partial.Request} {entities : Partial.Entities} {v : Spec.Value} {subsmap : Map Unknown Partial.Value}
+  (wf_r : req.AllWellFormed)
+  (wf_e : entities.AllWellFormed) :
+  req.subst subsmap = some req' →
+  Partial.evaluate expr req entities = .ok (.value v) →
+  Partial.evaluate (expr.subst subsmap) req' (entities.subst subsmap) = .ok (.value v)
+:= by
+  cases expr
+  case lit p =>
+    unfold Partial.evaluate
+    simp
+    intro _ h₁ ; subst h₁
+    simp [Partial.Expr.subst]
+  case var v => exact Var.subst_preserves_evaluation_to_value wf_r
+  case unknown u => unfold Partial.evaluate ; simp
+  case and x₁ x₂ =>
+    intro h_req h₁
+    have h₂ := And.evals_to_concrete_then_operands_eval_to_concrete (by
+      unfold EvaluatesToConcrete
+      exists v
+    )
+    unfold EvaluatesToConcrete at h₂
+    rcases h₂ with h₂ | ⟨⟨v₁, hx₁⟩, ⟨v₂, hx₂⟩⟩
+    · have ih := subst_preserves_evaluation_to_value wf_r wf_e h_req h₂
+      unfold Partial.Expr.subst Partial.evaluate Spec.Value.asBool
+      simp [ih]
+      unfold Partial.evaluate Spec.Value.asBool at h₁
+      simp [h₂] at h₁
+      exact h₁
+    · have ih₁ := subst_preserves_evaluation_to_value wf_r wf_e h_req hx₁
+      have ih₂ := subst_preserves_evaluation_to_value wf_r wf_e h_req hx₂
+      apply (AndOr.subst_preserves_evaluation_to_value _ _).left h_req v h₁
+      · unfold SubstPreservesEvaluationToConcrete
+        intro _ v₁' hx₁'
+        simp [hx₁'] at hx₁ ; subst v₁'
+        exact ih₁
+      · unfold SubstPreservesEvaluationToConcrete
+        intro _ v₂' hx₂'
+        simp [hx₂'] at hx₂ ; subst v₂'
+        exact ih₂
+  case or x₁ x₂ =>
+    intro h_req h₁
+    have h₂ := Or.evals_to_concrete_then_operands_eval_to_concrete (by
+      unfold EvaluatesToConcrete
+      exists v
+    )
+    unfold EvaluatesToConcrete at h₂
+    rcases h₂ with h₂ | ⟨⟨v₁, hx₁⟩, ⟨v₂, hx₂⟩⟩
+    · have ih := subst_preserves_evaluation_to_value wf_r wf_e h_req h₂
+      unfold Partial.Expr.subst Partial.evaluate Spec.Value.asBool
+      simp [ih]
+      unfold Partial.evaluate Spec.Value.asBool at h₁
+      simp [h₂] at h₁
+      exact h₁
+    · have ih₁ := subst_preserves_evaluation_to_value wf_r wf_e h_req hx₁
+      have ih₂ := subst_preserves_evaluation_to_value wf_r wf_e h_req hx₂
+      apply (AndOr.subst_preserves_evaluation_to_value _ _).right h_req v h₁
+      · unfold SubstPreservesEvaluationToConcrete
+        intro _ v₁' hx₁'
+        simp [hx₁'] at hx₁ ; subst v₁'
+        exact ih₁
+      · unfold SubstPreservesEvaluationToConcrete
+        intro _ v₂' hx₂'
+        simp [hx₂'] at hx₂ ; subst v₂'
+        exact ih₂
+  case binaryApp op x₁ x₂ =>
+    intro h_req h₁
+    have h₂ := Binary.evals_to_concrete_then_operands_eval_to_concrete (by
+      unfold EvaluatesToConcrete
+      exists v
+    )
+    unfold EvaluatesToConcrete at h₂
+    have ⟨⟨v₁, hx₁⟩, ⟨v₂, hx₂⟩⟩ := h₂ ; clear h₂
+    have ih₁ := subst_preserves_evaluation_to_value wf_r wf_e h_req hx₁
+    have ih₂ := subst_preserves_evaluation_to_value wf_r wf_e h_req hx₂
+    apply Binary.subst_preserves_evaluation_to_value _ _ h_req v h₁
+    · unfold SubstPreservesEvaluationToConcrete
+      intro _ v₁' hx₁'
+      simp [hx₁'] at hx₁ ; subst v₁'
+      exact ih₁
+    · unfold SubstPreservesEvaluationToConcrete
+      intro _ v₂' hx₂'
+      simp [hx₂'] at hx₂ ; subst v₂'
+      exact ih₂
+  case unaryApp op x₁ =>
+    intro h_req h₁
+    have h₂ := Unary.evals_to_concrete_then_operand_evals_to_concrete (by
+      unfold EvaluatesToConcrete
+      exists v
+    )
+    unfold EvaluatesToConcrete at h₂
+    have ⟨v₁, hx₁⟩ := h₂ ; clear h₂
+    have ih₁ := subst_preserves_evaluation_to_value wf_r wf_e h_req hx₁
+    apply Unary.subst_preserves_evaluation_to_value _ h_req v h₁
+    · unfold SubstPreservesEvaluationToConcrete
+      intro _ v₁' hx₁'
+      simp [hx₁'] at hx₁ ; subst v₁'
+      exact ih₁
+  case ite x₁ x₂ x₃ =>
+    intro h_req h₁
+    have h₂ := Ite.evals_to_concrete_then_operands_eval_to_concrete (by
+      unfold EvaluatesToConcrete
+      exists v
+    )
+    unfold EvaluatesToConcrete at h₂
+    rcases h₂ with ⟨hx₁, ⟨v₂, hx₂⟩⟩ | ⟨hx₁, ⟨v₃, hx₃⟩⟩
+    · have ih₁ := subst_preserves_evaluation_to_value wf_r wf_e h_req hx₁
+      have ih₂ := subst_preserves_evaluation_to_value wf_r wf_e h_req hx₂
+      apply Ite.subst_preserves_evaluation_to_value _ _ h_req v h₁
+      · unfold SubstPreservesEvaluationToConcrete
+        intro _ v₁' hx₁'
+        simp [hx₁'] at hx₁ ; subst v₁'
+        exact ih₁
+      · unfold SubstPreservesEvaluationToConcrete
+        left
+        apply And.intro hx₁
+        intro _ v₂' hx₂'
+        simp [hx₂'] at hx₂ ; subst v₂'
+        exact ih₂
+    · have ih₁ := subst_preserves_evaluation_to_value wf_r wf_e h_req hx₁
+      have ih₃ := subst_preserves_evaluation_to_value wf_r wf_e h_req hx₃
+      apply Ite.subst_preserves_evaluation_to_value _ _ h_req v h₁
+      · unfold SubstPreservesEvaluationToConcrete
+        intro _ v₁' hx₁'
+        simp [hx₁'] at hx₁ ; subst v₁'
+        exact ih₁
+      · unfold SubstPreservesEvaluationToConcrete
+        right
+        apply And.intro hx₁
+        intro _ v₃' hx₃'
+        simp [hx₃'] at hx₃ ; subst v₃'
+        exact ih₃
+  case getAttr x₁ attr =>
+    intro h_req h₁
+    have h₂ := GetAttr.evals_to_concrete_then_operand_evals_to_concrete (by
+      unfold EvaluatesToConcrete
+      exists v
+    )
+    unfold EvaluatesToConcrete at h₂
+    have ⟨v₁, hx₁⟩ := h₂ ; clear h₂
+    have ih₁ := subst_preserves_evaluation_to_value wf_r wf_e h_req hx₁
+    apply GetAttr.subst_preserves_evaluation_to_value wf_e _ h_req v h₁
+    · unfold SubstPreservesEvaluationToConcrete
+      intro _ v₁' hx₁'
+      simp [hx₁'] at hx₁ ; subst v₁'
+      exact ih₁
+  case hasAttr x₁ attr =>
+    intro h_req h₁
+    have h₂ := HasAttr.evals_to_concrete_then_operand_evals_to_concrete (by
+      unfold EvaluatesToConcrete
+      exists v
+    )
+    unfold EvaluatesToConcrete at h₂
+    have ⟨v₁, hx₁⟩ := h₂ ; clear h₂
+    have ih₁ := subst_preserves_evaluation_to_value wf_r wf_e h_req hx₁
+    apply HasAttr.subst_preserves_evaluation_to_value wf_e _ h_req v h₁
+    · unfold SubstPreservesEvaluationToConcrete
+      intro _ v₁' hx₁'
+      simp [hx₁'] at hx₁ ; subst v₁'
+      exact ih₁
+  case set xs =>
+    intro h_req h₁
+    have hx := Set.evals_to_concrete_then_elts_eval_to_concrete (by
+      unfold EvaluatesToConcrete
+      exists v
+    )
+    unfold EvaluatesToConcrete at hx
+    have ih : ∀ x ∈ xs, SubstPreservesEvaluationToConcrete x req req' entities subsmap := by
+      unfold SubstPreservesEvaluationToConcrete
+      intro x h₂ _ v' hx'
+      replace ⟨v, hx⟩ := hx x h₂
+      simp [hx] at hx' ; subst v'
+      have := List.sizeOf_lt_of_mem h₂
+      exact subst_preserves_evaluation_to_value wf_r wf_e h_req hx
+    exact Set.subst_preserves_evaluation_to_value ih h_req v h₁
+  case record attrs =>
+    intro h_req h₁
+    have hx := Record.evals_to_concrete_then_vals_eval_to_concrete (by
+      unfold EvaluatesToConcrete
+      exists v
+    )
+    unfold EvaluatesToConcrete at hx
+    have ih: ∀ kv ∈ attrs, SubstPreservesEvaluationToConcrete kv.snd req req' entities subsmap := by
+      unfold SubstPreservesEvaluationToConcrete
+      intro (k, x) h₂ _ v' hx'
+      replace ⟨v, hx⟩ := hx (k, x) h₂
+      simp [hx] at hx' ; subst v'
+      have := Map.sizeOf_lt_of_value h₂
+      exact subst_preserves_evaluation_to_value wf_r wf_e h_req hx
+    exact Record.subst_preserves_evaluation_to_value ih h_req v h₁
+  case call xfn xs =>
+    intro h_req h₁
+    have hx := Call.evals_to_concrete_then_args_eval_to_concrete (by
+      unfold EvaluatesToConcrete
+      exists v
+    )
+    unfold EvaluatesToConcrete at hx
+    have ih : ∀ x ∈ xs, SubstPreservesEvaluationToConcrete x req req' entities subsmap := by
+      unfold SubstPreservesEvaluationToConcrete
+      intro x h₂ _ v' hx'
+      replace ⟨v, hx⟩ := hx x h₂
+      simp [hx] at hx' ; subst v'
+      have := List.sizeOf_lt_of_mem h₂
+      exact subst_preserves_evaluation_to_value wf_r wf_e h_req hx
+    exact Call.subst_preserves_evaluation_to_value ih h_req v h₁
+termination_by expr
