cedar-lean/Cedar/Thm/Partial/Evaluation/AndOr.lean
@@ -1,0 +1,75 @@
+/-
+ Copyright Cedar Contributors
+
+ Licensed under the Apache License, Version 2.0 (the "License");
+ you may not use this file except in compliance with the License.
+ You may obtain a copy of the License at
+
+      https://www.apache.org/licenses/LICENSE-2.0
+
+ Unless required by applicable law or agreed to in writing, software
+ distributed under the License is distributed on an "AS IS" BASIS,
+ WITHOUT WARRANTIES OR CONDITIONS OF ANY KIND, either express or implied.
+ See the License for the specific language governing permissions and
+ limitations under the License.
+-/
+
+import Cedar.Partial.Evaluator
+import Cedar.Thm.Data.Control
+import Cedar.Thm.Partial.Evaluation.Basic
+
+namespace Cedar.Thm.Partial.Evaluation.AndOr
+
+open Cedar.Data
+open Cedar.Partial (Unknown)
+
+/- ## Lemmas shared by And.lean and Or.lean -/
+
+/--
+  Inductive argument that if partial-evaluation of a `Partial.Expr.and` or
+  `Partial.Expr.or` returns a concrete value, then it returns the same value
+  after any substitution of unknowns
+-/
+theorem subst_preserves_evaluation_to_value {x₁ x₂ : Partial.Expr} {req req' : Partial.Request} {entities : Partial.Entities} {subsmap : Map Unknown Partial.Value}
+  (ih₁ : SubstPreservesEvaluationToConcrete x₁ req req' entities subsmap)
+  (ih₂ : SubstPreservesEvaluationToConcrete x₂ req req' entities subsmap) :
+  SubstPreservesEvaluationToConcrete (Partial.Expr.and x₁ x₂) req req' entities subsmap ∧
+  SubstPreservesEvaluationToConcrete (Partial.Expr.or x₁ x₂) req req' entities subsmap
+:= by
+  unfold SubstPreservesEvaluationToConcrete at *
+  unfold Partial.evaluate Spec.Value.asBool
+  constructor
+  all_goals {
+    intro h_req v
+    specialize ih₁ h_req
+    specialize ih₂ h_req
+    unfold Partial.Expr.subst
+    cases hx₁ : Partial.evaluate x₁ req entities
+    <;> cases hx₂ : Partial.evaluate x₂ req entities
+    <;> simp [hx₁, hx₂] at *
+    case ok.ok pval₁ pval₂ =>
+      cases pval₁ <;> cases pval₂ <;> simp at *
+      case value.value v₁ v₂ =>
+        simp [ih₁, ih₂]
+      case value.residual v₁ r₂ =>
+        simp [ih₁]
+        cases v₁
+        case prim p₁ =>
+          cases p₁ <;> simp
+          case bool b₁ => cases b₁ <;> simp
+        case set s | record m => simp
+        case ext x => cases x <;> simp
+    case ok.error pval₁ e₂ =>
+      cases pval₁ <;> simp at *
+      case value v₁ =>
+        cases v₁
+        case prim p₁ =>
+          cases p₁ <;> simp
+          case bool b₁ =>
+            cases b₁ <;> simp <;> intro h₁ <;> subst v
+            simp [ih₁]
+        case set s | record m => simp
+        case ext x => cases x <;> simp
+  }
+
+end Cedar.Thm.Partial.Evaluation.AndOr
