cedar-lean/Cedar/Thm/Partial/Evaluation/Binary.lean
@@ -20,10 +20,12 @@ import Cedar.Thm.Data.Control
 import Cedar.Thm.Data.Map
 import Cedar.Thm.Data.Set
 import Cedar.Thm.Partial.Evaluation.Basic
+import Cedar.Thm.Partial.Subst
 
 namespace Cedar.Thm.Partial.Evaluation.Binary
 
 open Cedar.Data
+open Cedar.Partial (Unknown)
 open Cedar.Spec (BinaryOp EntityUID intOrErr Result)
 
 /--
@@ -104,5 +106,139 @@ theorem on_concrete_eqv_concrete_eval {x₁ x₂ : Spec.Expr} {request : Spec.Re
   case ok v₁ =>
     cases h₂ : Spec.evaluate x₂ request entities <;> simp only [h₂, Except.bind_err, Except.bind_ok]
     case ok v₂ => simp [evaluateBinaryApp_on_concrete_eqv_concrete, Except.map]
+
+/--
+  If `Partial.evaluateBinaryApp` produces `ok` with a concrete value, then so
+  would partial-evaluating either of the operands
+-/
+theorem evaluateBinaryApp_returns_concrete_then_operands_eval_to_concrete {pval₁ pval₂ : Partial.Value} {op : BinaryOp} {entities : Partial.Entities} :
+  Partial.evaluateBinaryApp op pval₁ pval₂ entities = .ok (.value v) →
+  (∃ v₁, pval₁ = .value v₁) ∧ (∃ v₂, pval₂ = .value v₂)
+:= by
+  unfold Partial.evaluateBinaryApp
+  intro h₁
+  cases pval₁ <;> cases pval₂
+  case value.value v₁ v₂ =>
+    exact And.intro (by exists v₁) (by exists v₂)
+  case value.residual v₁ r₂ =>
+    cases v₁ <;> simp at h₁
+  case residual.value r₁ v₂ =>
+    cases v₂ <;> simp at h₁
+  case residual.residual r₁ r₂ =>
+    simp at h₁
+
+/--
+  If partial-evaluating a `Partial.Expr.binaryApp` produces `ok` with a concrete
+  value, then so would partial-evaluating either of the operands
+-/
+theorem evals_to_concrete_then_operands_eval_to_concrete {x₁ x₂ : Partial.Expr} {op : BinaryOp} {request : Partial.Request} {entities : Partial.Entities} :
+  EvaluatesToConcrete (Partial.Expr.binaryApp op x₁ x₂) request entities →
+  (EvaluatesToConcrete x₁ request entities ∧ EvaluatesToConcrete x₂ request entities)
+:= by
+  unfold EvaluatesToConcrete
+  intro h₁
+  unfold Partial.evaluate at h₁
+  replace ⟨v, h₁⟩ := h₁
+  cases hx₁ : Partial.evaluate x₁ request entities
+  <;> cases hx₂ : Partial.evaluate x₂ request entities
+  <;> simp [hx₁, hx₂] at h₁
+  case ok.ok pval₁ pval₂ =>
+    have ⟨⟨v₁, hv₁⟩, ⟨v₂, hv₂⟩⟩ := evaluateBinaryApp_returns_concrete_then_operands_eval_to_concrete h₁
+    subst pval₁ pval₂
+    exact And.intro (by exists v₁) (by exists v₂)
+
+/--
+  The return value of `Partial.inₑ` is not affected by substitution of unknowns
+  in `entities`
+-/
+theorem partialInₑ_subst_const {uid₁ uid₂ : EntityUID} {entities : Partial.Entities} {subsmap : Map Unknown Partial.Value} :
+  Partial.inₑ uid₁ uid₂ entities = Partial.inₑ uid₁ uid₂ (entities.subst subsmap)
+:= by
+  unfold Partial.inₑ
+  cases uid₁ == uid₂ <;> simp
+  case false =>
+    rw [← Partial.Subst.entities_subst_preserves_ancestorsOrEmpty entities uid₁ subsmap]
+
+/--
+  The return value of `Partial.inₛ` is not affected by substitution of unknowns
+  in `entities`
+-/
+theorem partialInₛ_subst_const {uid₁ : EntityUID} {s₂ : Set Spec.Value} {entities : Partial.Entities} {subsmap : Map Unknown Partial.Value} :
+  Partial.inₛ uid₁ s₂ entities = Partial.inₛ uid₁ s₂ (entities.subst subsmap)
+:= by
+  unfold Partial.inₛ
+  cases s₂.mapOrErr Spec.Value.asEntityUID .typeError <;> simp
+  case ok uids => simp [← partialInₑ_subst_const]
+
+/--
+  If `Partial.apply₂` returns a concrete value, then it returns the same value
+  after any substitution of unknowns in `entities`
+-/
+theorem partialApply₂_subst_preserves_evaluation_to_value {v₁ v₂ : Spec.Value} {op : BinaryOp} {entities : Partial.Entities} {subsmap : Map Unknown Partial.Value} :
+  Partial.apply₂ op v₁ v₂ entities = .ok (.value v) →
+  Partial.apply₂ op v₁ v₂ (entities.subst subsmap) = .ok (.value v)
+:= by
+  unfold Partial.apply₂
+  cases op
+  case eq => simp
+  case mem =>
+    cases v₁ <;> cases v₂
+    case prim.prim p₁ p₂ =>
+      cases p₁ <;> cases p₂ <;> simp
+      case entityUID.entityUID uid₁ uid₂ =>
+        rw [← partialInₑ_subst_const]
+        simp
+    case prim.set p₁ s₂ =>
+      cases p₁ <;> simp
+      case entityUID uid₁ =>
+        rw [← partialInₛ_subst_const]
+        simp
+    all_goals simp
+  all_goals {
+    cases v₁ <;> cases v₂
+    case prim.prim p₁ p₂ =>
+      cases p₁ <;> cases p₂ <;> simp
+    all_goals simp
+  }
+
+/--
+  If `Partial.evaluateBinaryApp` returns a concrete value, then it returns
+  the same value after any substitution of unknowns in `entities`
+-/
+theorem evaluateBinaryApp_subst_preserves_evaluation_to_value {pval₁ pval₂ : Partial.Value} {op : BinaryOp} {entities : Partial.Entities} {subsmap : Map Unknown Partial.Value} :
+  Partial.evaluateBinaryApp op pval₁ pval₂ entities = .ok (.value v) →
+  Partial.evaluateBinaryApp op pval₁ pval₂ (entities.subst subsmap) = .ok (.value v)
+:= by
+  unfold Partial.evaluateBinaryApp
+  cases pval₁ <;> cases pval₂ <;> simp
+  case value.value v₁ v₂ => exact partialApply₂_subst_preserves_evaluation_to_value
+
+/--
+  Inductive argument that if partial-evaluation of a `Partial.Expr.binaryApp`
+  returns a concrete value, then it returns the same value after any
+  substitution of unknowns
+-/
+theorem subst_preserves_evaluation_to_value {x₁ x₂ : Partial.Expr} {op : BinaryOp} {req req' : Partial.Request} {entities : Partial.Entities} {subsmap : Map Unknown Partial.Value}
+  (ih₁ : SubstPreservesEvaluationToConcrete x₁ req req' entities subsmap)
+  (ih₂ : SubstPreservesEvaluationToConcrete x₂ req req' entities subsmap) :
+  SubstPreservesEvaluationToConcrete (Partial.Expr.binaryApp op x₁ x₂) req req' entities subsmap
+:= by
+  unfold SubstPreservesEvaluationToConcrete at *
+  unfold Partial.evaluate Spec.Value.asBool
+  intro h_req v
+  specialize ih₁ h_req
+  specialize ih₂ h_req
+  unfold Partial.Expr.subst
+  cases hx₁ : Partial.evaluate x₁ req entities
+  <;> cases hx₂ : Partial.evaluate x₂ req entities
+  <;> simp [hx₁, hx₂] at *
+  case ok.ok pval₁ pval₂ =>
+    cases pval₁ <;> cases pval₂ <;> simp at *
+    case value.value v₁ v₂ =>
+      simp [ih₁, ih₂]
+      exact evaluateBinaryApp_subst_preserves_evaluation_to_value
+    case value.residual v₁ r₂ => simp [Partial.evaluateBinaryApp]
+    case residual.value r₁ v₂ => simp [Partial.evaluateBinaryApp]
+    case residual.residual r₁ r₂ => simp [Partial.evaluateBinaryApp]
 
 end Cedar.Thm.Partial.Evaluation.Binary
