cedar-lean/Cedar/Thm/Partial/Evaluation/Ite.lean
@@ -21,6 +21,8 @@ import Cedar.Thm.Partial.Evaluation.Basic
 
 namespace Cedar.Thm.Partial.Evaluation.Ite
 
+open Cedar.Data
+open Cedar.Partial (Unknown)
 open Cedar.Spec (Result)
 
 /--
@@ -46,5 +48,74 @@ theorem on_concrete_eqv_concrete_eval {x₁ x₂ x₃ : Spec.Expr} {request : Sp
     case prim p =>
       cases p <;> simp only [Except.bind_ok, Except.bind_err]
       case bool b => cases b <;> simp
+
+/--
+  If partial-evaluating a `Partial.Expr.ite` produces `ok` with a concrete
+  value, then so would partial-evaluating any of the operands, unless the `ite`
+  short-circuits
+-/
+theorem evals_to_concrete_then_operands_eval_to_concrete {x₁ x₂ x₃ : Partial.Expr} {request : Partial.Request} {entities : Partial.Entities} :
+  EvaluatesToConcrete (Partial.Expr.ite x₁ x₂ x₃) request entities →
+  (Partial.evaluate x₁ request entities = .ok (.value (.prim (.bool true))) ∧ EvaluatesToConcrete x₂ request entities) ∨
+  (Partial.evaluate x₁ request entities = .ok (.value (.prim (.bool false))) ∧ EvaluatesToConcrete x₃ request entities)
+:= by
+  unfold EvaluatesToConcrete
+  intro h₁
+  unfold Partial.evaluate at h₁
+  replace ⟨v, h₁⟩ := h₁
+  cases hx₁ : Partial.evaluate x₁ request entities
+  <;> simp [hx₁, Spec.Value.asBool] at h₁
+  case ok pval₁ =>
+    cases pval₁ <;> simp at h₁
+    case value v₁ =>
+      cases v₁
+      case prim p₁ =>
+        cases p₁ <;> simp at h₁
+        case bool b₁ =>
+          cases b₁ <;> simp at h₁
+          case true =>
+            left
+            cases hx₂ : Partial.evaluate x₂ request entities
+            <;> simp [hx₂] at h₁
+            case ok v₂ => subst h₁ ; simp
+          case false =>
+            right
+            cases hx₃ : Partial.evaluate x₃ request entities
+            <;> simp [hx₃] at h₁
+            case ok v₃ => subst h₁ ; simp
+      case set s | record m => simp at h₁
+      case ext x => cases x <;> simp at h₁
+
+/--
+  Inductive argument that if partial-evaluation of a `Partial.Expr.ite` returns
+  a concrete value, then it returns the same value after any substitution of
+  unknowns
+-/
+theorem subst_preserves_evaluation_to_value {x₁ x₂ x₃ : Partial.Expr} {req req' : Partial.Request} {entities : Partial.Entities} {subsmap : Map Unknown Partial.Value}
+  (ih₁ : SubstPreservesEvaluationToConcrete x₁ req req' entities subsmap)
+  (ih₂₃ :
+    (Partial.evaluate x₁ req entities = .ok (.value (.prim (.bool true))) ∧ SubstPreservesEvaluationToConcrete x₂ req req' entities subsmap) ∨
+    (Partial.evaluate x₁ req entities = .ok (.value (.prim (.bool false))) ∧ SubstPreservesEvaluationToConcrete x₃ req req' entities subsmap)
+  ) :
+  SubstPreservesEvaluationToConcrete (Partial.Expr.ite x₁ x₂ x₃) req req' entities subsmap
+:= by
+  unfold SubstPreservesEvaluationToConcrete Partial.evaluate Spec.Value.asBool
+  intro h_req v
+  specialize ih₁ h_req
+  rcases ih₂₃ with ⟨hx₁, ih₂⟩ | ⟨hx₁, ih₃⟩
+  · specialize ih₂ h_req
+    specialize ih₁ (.prim (.bool true)) hx₁
+    unfold Partial.Expr.subst
+    simp [hx₁]
+    intro h₁
+    simp [ih₁]
+    exact ih₂ v h₁
+  · specialize ih₃ h_req
+    specialize ih₁ (.prim (.bool false)) hx₁
+    unfold Partial.Expr.subst
+    simp [hx₁]
+    intro h₁
+    simp [ih₁]
+    exact ih₃ v h₁
 
 end Cedar.Thm.Partial.Evaluation.Ite
