cedar-lean/Cedar/Thm/Partial/Evaluation/Unary.lean
@@ -21,13 +21,15 @@ import Cedar.Thm.Partial.Evaluation.Basic
 
 namespace Cedar.Thm.Partial.Evaluation.Unary
 
+open Cedar.Data
+open Cedar.Partial (Unknown)
 open Cedar.Spec (UnaryOp)
 
 /--
   `Partial.apply₁` on concrete arguments gives the same output as `Spec.apply₁`
   on the same arguments
 -/
-theorem apply₁_on_concrete_eqv_concrete {op : UnaryOp} {v : Spec.Value} :
+theorem apply₁_on_concrete_eqv_concrete (op : UnaryOp) (v : Spec.Value) :
   Partial.apply₁ op v = (Spec.apply₁ op v).map Partial.Value.value
 := by
   rfl
@@ -48,5 +50,59 @@ theorem on_concrete_eqv_concrete_eval {x₁ : Spec.Expr} {request : Spec.Request
   cases Spec.evaluate x₁ request entities <;> simp only [Except.bind_err, Except.bind_ok]
   case error e => simp [Except.map]
   case ok v₁ => rfl
+
+/--
+  If `Partial.apply₁` produces `ok` with a concrete value, then so would
+  partial-evaluating its operand
+-/
+theorem partialApply₁_returns_concrete_then_operand_evals_to_concrete {pval₁ : Partial.Value} {op : UnaryOp} :
+  Partial.apply₁ op pval₁ = .ok (.value v) →
+  ∃ v₁, pval₁ = .value v₁
+:= by
+  unfold Partial.apply₁
+  intro h₁
+  cases pval₁
+  case value v₁ => exists v₁
+  case residual r₁ => simp at h₁
+
+/--
+  If partial-evaluating a `Partial.Expr.unaryApp` produces `ok` with a concrete
+  value, then so would partial-evaluating its operand
+-/
+theorem evals_to_concrete_then_operand_evals_to_concrete {x₁ : Partial.Expr} {op : UnaryOp} {request : Partial.Request} {entities : Partial.Entities} :
+  EvaluatesToConcrete (Partial.Expr.unaryApp op x₁) request entities →
+  EvaluatesToConcrete x₁ request entities
+:= by
+  unfold EvaluatesToConcrete
+  intro h₁
+  unfold Partial.evaluate at h₁
+  replace ⟨v, h₁⟩ := h₁
+  cases hx₁ : Partial.evaluate x₁ request entities
+  <;> simp [hx₁] at h₁
+  case ok pval₁ =>
+    have ⟨v₁, hv₁⟩ := partialApply₁_returns_concrete_then_operand_evals_to_concrete h₁
+    subst pval₁
+    exists v₁
+
+/--
+  Inductive argument that if partial-evaluation of a `Partial.Expr.unaryApp`
+  returns a concrete value, then it returns the same value after any
+  substitution of unknowns
+-/
+theorem subst_preserves_evaluation_to_value {x₁ : Partial.Expr} {op : UnaryOp} {req req' : Partial.Request} {entities : Partial.Entities} {subsmap : Map Unknown Partial.Value}
+  (ih₁ : SubstPreservesEvaluationToConcrete x₁ req req' entities subsmap) :
+  SubstPreservesEvaluationToConcrete (Partial.Expr.unaryApp op x₁) req req' entities subsmap
+:= by
+  unfold SubstPreservesEvaluationToConcrete at *
+  unfold Partial.evaluate Spec.Value.asBool
+  intro h_req v
+  specialize ih₁ h_req
+  unfold Partial.Expr.subst
+  cases hx₁ : Partial.evaluate x₁ req entities
+  <;> simp [hx₁] at *
+  case ok pval₁ =>
+    cases pval₁ <;> simp at *
+    case value v₁ => simp [ih₁]
+    case residual r₁ => simp [Partial.apply₁]
 
 end Cedar.Thm.Partial.Evaluation.Unary
