cedar-lean/Cedar/Thm/Partial/Subst.lean
@@ -15,10 +15,14 @@
 -/
 
 import Cedar.Data.Map
+import Cedar.Partial.Entities
 import Cedar.Partial.Expr
+import Cedar.Partial.Request
 import Cedar.Partial.Value
 import Cedar.Spec.Expr
 import Cedar.Thm.Data.List
+import Cedar.Thm.Data.LT
+import Cedar.Thm.Partial.Evaluation.Basic
 
 /-! ## Lemmas about `subst` operations -/
 
@@ -26,6 +30,7 @@ namespace Cedar.Thm.Partial.Subst
 
 open Cedar.Data
 open Cedar.Partial (Unknown)
+open Cedar.Spec (Attr EntityUID)
 
 /--
   subst on a concrete expression is that expression
@@ -119,3 +124,252 @@ decreasing_by
     have h₃ := Map.sizeOf_lt_of_kvs m
     simp [Map.kvs] at h₂ h₃
     omega
+
+/--
+  Partial.Value.subst preserves well-formedness
+-/
+theorem val_subst_preserves_wf {v v' : Partial.Value} {subsmap : Map Unknown Partial.Value} :
+  v.WellFormed →
+  v.subst subsmap = some v' →
+  v'.WellFormed
+:= by
+  unfold Partial.Value.WellFormed Partial.Value.subst
+  cases v <;> simp
+  case value v =>
+    intro h₁ h₂
+    subst h₂
+    simp [h₁]
+  case residual r =>
+    intro h₁
+    subst h₁
+    simp
+
+/--
+  Partial.Request.subst preserves well-formedness
+-/
+theorem req_subst_preserves_wf {req req' : Partial.Request} {subsmap : Map Unknown Partial.Value} :
+  req.AllWellFormed →
+  req.subst subsmap = some req' →
+  req'.AllWellFormed
+:= by
+  unfold Partial.Request.AllWellFormed Partial.Request.subst
+  intro wf h₁
+  have ⟨wf_c, wf_vals⟩ := wf ; clear wf
+  simp at h₁
+  replace ⟨principal, _, ⟨action, _, ⟨resource, _, h₁⟩⟩⟩ := h₁
+  subst h₁
+  simp
+  apply And.intro (Map.mapOnValues_wf.mp wf_c)
+  intro pval' h₁
+  rw [Map.values_mapOnValues] at h₁
+  replace ⟨pval, h₁, h₂⟩ := List.mem_map.mp h₁
+  subst pval'
+  apply val_subst_preserves_wf (wf_vals pval h₁) (subsmap := subsmap)
+  rfl
+
+/--
+  Partial.Request.subst preserves a known principal UID
+-/
+theorem req_subst_preserves_known_principal {req req' : Partial.Request} {uid : EntityUID} {subsmap : Map Unknown Partial.Value} :
+  req.principal = .known uid →
+  req.subst subsmap = some req' →
+  req'.principal = .known uid
+:= by
+  intro h₁ h_req
+  simp [Partial.Request.subst] at h_req
+  replace ⟨principal, h_p, ⟨action, _, ⟨resource, _, h_req⟩⟩⟩ := h_req
+  subst req'
+  simp only
+  simp [h₁, Partial.UidOrUnknown.subst] at h_p
+  exact h_p.symm
+
+/--
+  Partial.Request.subst preserves a known action UID
+-/
+theorem req_subst_preserves_known_action {req req' : Partial.Request} {uid : EntityUID} {subsmap : Map Unknown Partial.Value} :
+  req.action = .known uid →
+  req.subst subsmap = some req' →
+  req'.action = .known uid
+:= by
+  intro h₁ h_req
+  simp [Partial.Request.subst] at h_req
+  replace ⟨principal, _, ⟨action, h_a, ⟨resource, _, h_req⟩⟩⟩ := h_req
+  subst req'
+  simp only
+  simp [h₁, Partial.UidOrUnknown.subst] at h_a
+  exact h_a.symm
+
+/--
+  Partial.Request.subst preserves a known resource UID
+-/
+theorem req_subst_preserves_known_resource {req req' : Partial.Request} {uid : EntityUID} {subsmap : Map Unknown Partial.Value} :
+  req.resource = .known uid →
+  req.subst subsmap = some req' →
+  req'.resource = .known uid
+:= by
+  intro h₁ h_req
+  simp [Partial.Request.subst] at h_req
+  replace ⟨principal, _, ⟨action, _, ⟨resource, h_r, h_req⟩⟩⟩ := h_req
+  subst req'
+  simp only
+  simp [h₁, Partial.UidOrUnknown.subst] at h_r
+  exact h_r.symm
+
+/--
+  Partial.Request.subst preserves the keyset of `context`
+-/
+theorem req_subst_preserves_keys_of_context {req req' : Partial.Request} {subsmap : Map Unknown Partial.Value} :
+  req.subst subsmap = some req' →
+  req.context.keys = req'.context.keys
+:= by
+  unfold Partial.Request.subst
+  simp only [Option.bind_eq_bind, Option.bind_eq_some, Option.some.injEq, forall_exists_index,
+    and_imp]
+  intro p _ a _ r _ _
+  subst req' ; simp only
+  exact (Map.keys_mapOnValues (Partial.Value.subst subsmap) req.context).symm
+
+/--
+  Partial.Request.subst preserves concrete values in the `context`
+-/
+theorem req_subst_preserves_concrete_context_vals {req req' : Partial.Request} {k : Attr} {subsmap : Map Unknown Partial.Value} :
+  (k, .value v) ∈ req.context.kvs →
+  req.subst subsmap = some req' →
+  (k, .value v) ∈ req'.context.kvs
+:= by
+  unfold Partial.Request.subst
+  simp
+  intro h₁ p _ a _ r _ h₂
+  subst req'
+  simp
+  rw [← subst_concrete_value v subsmap]
+  exact Map.in_kvs_in_mapOnValues h₁
+
+/--
+  Partial.EntityData.subst preserves well-formedness
+-/
+theorem entitydata_subst_preserves_wf {ed : Partial.EntityData} (subsmap : Map Unknown Partial.Value) :
+  ed.WellFormed → (ed.subst subsmap).WellFormed
+:= by
+  unfold Partial.EntityData.WellFormed Partial.EntityData.subst
+  intro h₁
+  simp only
+  and_intros
+  · exact Map.mapOnValues_wf.mp h₁.left
+  · exact h₁.right
+
+/--
+  Partial.Entities.subst preserves well-formedness
+-/
+theorem entities_subst_preserves_wf {entities : Partial.Entities} (subsmap : Map Unknown Partial.Value) :
+  entities.AllWellFormed → (entities.subst subsmap).AllWellFormed
+:= by
+  unfold Partial.Entities.AllWellFormed Partial.Entities.subst
+  intro h₁
+  constructor
+  · exact Map.mapOnValues_wf.mp h₁.left
+  · intro ed' h₂
+    simp [Map.values_mapOnValues] at h₂
+    replace ⟨ed, h₂, h₃⟩ := h₂
+    subst ed'
+    exact entitydata_subst_preserves_wf subsmap (h₁.right ed h₂)
+
+/--
+  Partial.EntityData.subst preserves .ancestors
+-/
+theorem entitydata_subst_preserves_ancestors (ed : Partial.EntityData) (subsmap : Map Unknown Partial.Value) :
+  ed.ancestors = (ed.subst subsmap).ancestors
+:= by
+  simp [Partial.EntityData.subst]
+
+/--
+  Partial.EntityData.subst preserves .contains on .attrs
+-/
+theorem entitydata_subst_preserves_contains_on_attrs (ed : Partial.EntityData) (attr : Attr) (subsmap : Map Unknown Partial.Value)
+  (wf : ed.WellFormed) :
+  ed.attrs.contains attr = (ed.subst subsmap).attrs.contains attr
+:= by
+  simp [Partial.EntityData.subst]
+  unfold Partial.EntityData.WellFormed at wf
+  apply Eq.symm
+  cases h₁ : ed.attrs.contains attr
+  case false =>
+    rw [← Bool.not_eq_true] at *
+    rw [Map.contains_iff_some_find?] at *
+    simp at *
+    intro pval h₂
+    conv at h₁ => intro pval ; rw [← Map.in_list_iff_find?_some wf.left]
+    rw [← Map.in_list_iff_find?_some (Map.mapOnValues_wf.mp wf.left)] at h₂
+    simp [Map.mapOnValues, Map.kvs] at h₂
+    replace ⟨(attr', pval'), h₂, h₃, h₄⟩ := h₂
+    subst h₃ h₄
+    simp [Map.kvs] at h₁
+    exact h₁ pval' h₂
+  case true =>
+    rw [Map.contains_iff_some_find?] at *
+    replace ⟨pval, h₁⟩ := h₁
+    rw [← Map.in_list_iff_find?_some wf.left] at h₁
+    exists (pval.subst subsmap)
+    rw [← Map.in_list_iff_find?_some (Map.mapOnValues_wf.mp wf.left)]
+    simp [Map.mapOnValues, Map.kvs]
+    exists (attr, pval)
+
+/--
+  Partial.EntityData.subst preserves concrete attribute values
+-/
+theorem entitydata_subst_preserves_concrete_attrs {ed : Partial.EntityData} (subsmap : Map Unknown Partial.Value) :
+  (k, .value v) ∈ ed.attrs.kvs → (k, .value v) ∈ (ed.subst subsmap).attrs.kvs
+:= by
+  simp [Partial.EntityData.subst]
+  intro h₁
+  rw [← subst_concrete_value v subsmap]
+  exact Map.in_kvs_in_mapOnValues h₁
+
+/--
+  Partial.Entities.subst preserves .ancestorsOrEmpty
+-/
+theorem entities_subst_preserves_ancestorsOrEmpty (entities : Partial.Entities) (uid : EntityUID) (subsmap : Map Unknown Partial.Value) :
+  entities.ancestorsOrEmpty uid = (entities.subst subsmap).ancestorsOrEmpty uid
+:= by
+  unfold Partial.Entities.subst Partial.Entities.ancestorsOrEmpty
+  cases h₁ : entities.find? uid
+  case none => simp [Map.find?_mapOnValues_none _ h₁]
+  case some ed =>
+    simp [Map.find?_mapOnValues_some _ h₁]
+    exact entitydata_subst_preserves_ancestors ed subsmap
+
+/--
+  Partial.Entities.subst preserves concrete attribute values
+-/
+theorem entities_subst_preserves_concrete_attrs {entities : Partial.Entities} {uid : EntityUID} (subsmap : Map Unknown Partial.Value) :
+  entities.attrs uid = .ok attrs →
+  (k, .value v) ∈ attrs.kvs →
+  ∃ attrs', (entities.subst subsmap).attrs uid = .ok attrs' ∧ (k, .value v) ∈ attrs'.kvs
+:= by
+  unfold Partial.Entities.subst Partial.Entities.attrs
+  cases h₁ : entities.findOrErr uid Spec.Error.entityDoesNotExist <;> simp
+  case ok ed =>
+    intro h h₂ ; subst h
+    have h₃ := entitydata_subst_preserves_concrete_attrs subsmap h₂
+    exists (ed.subst subsmap).attrs
+    apply And.intro _ h₃
+    simp [Map.findOrErr_mapOnValues]
+    simp [h₁, Except.map]
+
+/--
+  Partial.Entities.subst preserves `Map.contains` for the attrs maps
+-/
+theorem entities_subst_preserves_contains_on_attrsOrEmpty (entities : Partial.Entities) (uid : EntityUID) (attr : Attr) (subsmap : Map Unknown Partial.Value)
+  (wf : entities.AllWellFormed) :
+  (entities.attrsOrEmpty uid).contains attr = ((entities.subst subsmap).attrsOrEmpty uid).contains attr
+:= by
+  unfold Partial.Entities.subst Partial.Entities.attrsOrEmpty
+  cases h₁ : entities.find? uid
+  case none => simp [Map.find?_mapOnValues_none _ h₁]
+  case some ed =>
+    simp [Map.find?_mapOnValues_some _ h₁]
+    apply entitydata_subst_preserves_contains_on_attrs ed attr subsmap
+    unfold Partial.Entities.AllWellFormed at wf
+    apply wf.right
+    simp [← Map.in_list_iff_find?_some wf.left] at h₁
+    exact Map.in_list_in_values h₁
